scripts/mk_dec_eq.hs
@@ -1,0 +1,62 @@
+
+module MkDecEq where
+
+import Data.List
+
+type Type = [ (String, [Bool]) ]
+
+-- (ctore_name, args (True == is recursive))
+ctors =
+  [ ("bv", [False])
+  , ("bit", [])
+  , ("float", [])
+  , ("double", [])
+  , ("x86_80", [])
+  , ("vec", [False, True])
+  , ("pair", [True, True])
+  , ("fn"  , [True, True]) ]
+
+-- We need to produce two types of equation --- recursive and mismatch.  The mismatch cases are simple,
+-- if tedious, while the recursive cases are a bit trickier
+
+mismatch :: String -> Type -> [String]
+mismatch tname cons = [ doOne x y | x <- cons, y <- cons, x /= y ]
+  where
+    noConf = "isFalse (λh, " ++ tname ++ ".noConfusion h)"
+    underscores c 0 = c
+    underscores c n = "(" ++ c ++ " " ++ intercalate " " (replicate n "_") ++ ")"
+    doOne (c1, args1) (c2, args2) = "| "   ++ underscores c1 (length args1)
+                                    ++ " " ++ underscores c2 (length args2)
+                                    ++ " := " ++ noConf
+
+recursive :: String -> Type -> String -> [String]
+recursive tname cons recName = map doOne cons
+  where
+    ctor (c, [])   _   = c -- never called, included for completeness
+    ctor (c, args) sfx = "(" ++ c ++ " " ++ intercalate " " (map (\n -> "c" ++ show n ++ sfx) [1 .. length args]) ++ ")"
+    doOne (n, [])      = "| " ++ n ++ " " ++ n ++ " := isTrue rfl"
+    doOne c@(_, args)  = "| " ++ ctor c "" ++ " " ++ ctor c "'" ++ " := "
+                         ++ "\n (" ++ match c ++ "\n"
+                         ++ trueMatch (length args) ++ "\n"
+                         ++ intercalate "\n" (map (falseMatch (length args)) [1 .. length args]) ++ ")"
+    
+    match (c, cs)    = "match " ++ intercalate ", " (zipWith oneHdr cs [1..]) ++ " with "
+    oneHdr b n = (if b then recName else "decEq") ++ " c" ++ show n ++ " c" ++ show n ++ "'"
+    
+    hyps n sfx = map (\n -> "h" ++ show n ++ sfx) [1..n]
+    trueMatch n      =
+      "  | " ++ intercalate ", " (map (\h -> "(isTrue " ++ h ++ ")") (hyps n "")) ++ " := "
+             ++ "isTrue (" ++ intercalate " ▸ " (hyps n "" ++ ["rfl"]) ++ ")"
+
+    falseMatch n pos = "  | "
+      ++ intercalate ", " (replicate (pos - 1) "(isTrue _)" ++ ["(isFalse nh)"] ++ (replicate (n - pos) "_"))
+      ++ " := " ++ noConf n pos
+    noConf n pos = "isFalse (λh, " ++ tname ++ ".noConfusion h $ λ"
+                   ++ intercalate " " (hyps n "'") ++ ", absurd h" ++ show pos ++ "' nh)"
+
+mkDecEq :: String -> Type -> String -> String
+mkDecEq tname cons recName =
+  "protected def " ++ recName ++ " : Π(e e' : " ++ tname ++ "), Decidable (e = e')\n"
+  ++ intercalate "\n" (recursive tname cons recName ++ mismatch tname cons)
+
+  
