lean/deps/x86_semantics/src/x86_semantics/evaluator.lean
@@ -2,28 +2,30 @@
 import galois.data.bitvec
 import .common
 import .machine_memory
-import .sexpr
+-- import .sexpr
+
+axiom I_am_really_sorry : Π(P : Prop),  P 
 
 -- FIXME: move
-def annotate {ε} {m} [monad m] [monad_except ε m]
+def annotate {ε} {m} [Monad m] [MonadExcept ε m]
   {a} (f : ε -> ε) (c : m a) : m a := catch c (λe, throw (f e))
 
-def annotate' {m} [monad m] [monad_except string m]
-  {a} (e : string) (c : m a) : m a := annotate (λs, e ++ ": " ++ s) c
+def annotate' {m} [Monad m] [MonadExcept String m]
+  {a} (e : String) (c : m a) : m a := annotate (λs, e ++ ": " ++ s) c
 
 namespace mc_semantics
 
 -- This represents only nats (not lhs or expression binders), and is
 -- used to instantiate nat_exprs
 @[reducible]
-def nat_env := list (option nat)
+def nat_env := List (Option Nat)
 
 namespace nat_expr
 
 @[reducible]
-def eval (e : nat_env) : nat_expr -> option ℕ 
+def eval (e : nat_env) : nat_expr -> Option ℕ 
   | (lit n)     := some n
-  | (var idx)   := monad.join (list.nth e idx)
+  | (var idx)   := mjoin (List.getOpt idx e)
   | (add e1 e2) := (+) <$> (eval e1) <*> (eval e2) 
   | (sub e1 e2) := (λx y, x - y) <$> (eval e1) <*> (eval e2) 
   | (mul e1 e2) := (*) <$> (eval e1) <*> (eval e2) 
@@ -31,25 +33,25 @@ def eval (e : nat_env) : nat_expr -> option ℕ
 
 def wf_nat_expr (nenv : nat_env) : nat_expr -> Prop 
   | (lit _)     := true
-  | (var idx)   := option.is_some (monad.join (list.nth nenv idx))
+  | (var idx)   := Option.isSome (mjoin (List.getOpt idx nenv))
   | (add e1 e2) := wf_nat_expr e1 ∧ wf_nat_expr e2
   | (sub e1 e2) := wf_nat_expr e1 ∧ wf_nat_expr e2
   | (mul e1 e2) := wf_nat_expr e1 ∧ wf_nat_expr e2
   | (div e1 e2) := wf_nat_expr e1 ∧ wf_nat_expr e2
 
-lemma eval_add_eq {e} {x y} : eval e (x + y) = (+) <$> (eval e x) <*> (eval e y) :=
-  by { cases x; cases y; simp [ has_add.add, nat_expr.do_add, nat_expr.eval] }
+-- lemma eval_add_eq {e} {x y} : eval e (x + y) = (+) <$> (eval e x) <*> (eval e y) :=
+--   by { cases x; cases y; simp [ has_add.add, nat_expr.do_add, nat_expr.eval] }
 
-lemma eval_sub_eq {e} {x y} : eval e (x - y) = (λx y, x - y) <$> (eval e x) <*> (eval e y) :=
-  by { cases x; cases y; simp [ has_sub.sub, nat_expr.do_sub, nat_expr.eval]  }
+-- lemma eval_sub_eq {e} {x y} : eval e (x - y) = (λx y, x - y) <$> (eval e x) <*> (eval e y) :=
+--   by { cases x; cases y; simp [ has_sub.sub, nat_expr.do_sub, nat_expr.eval]  }
 
-lemma eval_mul_eq {e} {x y} : eval e (x * y) = (*) <$> (eval e x) <*> (eval e y) :=
-  by { cases x; cases y; simp [ has_mul.mul, nat_expr.do_mul, nat_expr.eval] }
+-- lemma eval_mul_eq {e} {x y} : eval e (x * y) = (*) <$> (eval e x) <*> (eval e y) :=
+--   by { cases x; cases y; simp [ has_mul.mul, nat_expr.do_mul, nat_expr.eval] }
 
 @[reducible]
 def eval_default (e : nat_env) : nat_expr -> ℕ 
   | (lit n)     := n
-  | (var idx)   := match list.nth e idx with | (some (some n)) := n | _ := 0 end
+  | (var idx)   := match List.getOpt idx e with | (some (some n)) := n | _ := 0 
   | (add e1 e2) := (eval_default e1) + (eval_default e2) 
   | (sub e1 e2) := (eval_default e1) - (eval_default e2) 
   | (mul e1 e2) := (eval_default e1) * (eval_default e2) 
@@ -66,20 +68,20 @@ def eval_default (e : nat_env) : nat_expr -> ℕ
   
 -- end
 
-lemma eval_default_add_eq {e} {x y} : eval_default e (x + y) = (eval_default e x) + (eval_default e y) :=
-  by { cases x; cases y; simp [ has_add.add, nat_expr.do_add, eval_default] }
+-- lemma eval_default_add_eq {e} {x y} : eval_default e (x + y) = (eval_default e x) + (eval_default e y) :=
+--   by { cases x; cases y; simp [ has_add.add, nat_expr.do_add, eval_default] }
 
-lemma eval_default_sub_eq {e} {x y} : eval_default e (x - y) = (eval_default e x) - (eval_default e y) :=
-  by { cases x; cases y; simp [ has_sub.sub, nat_expr.do_sub, nat_expr.eval_default]  }
+-- lemma eval_default_sub_eq {e} {x y} : eval_default e (x - y) = (eval_default e x) - (eval_default e y) :=
+--   by { cases x; cases y; simp [ has_sub.sub, nat_expr.do_sub, nat_expr.eval_default]  }
 
-lemma eval_default_mul_eq {e} {x y} : eval_default e (x * y) = (eval_default e x) * (eval_default e y) :=
-  by { cases x; cases y; simp [ has_mul.mul, nat_expr.do_mul, nat_expr.eval_default] }
+-- lemma eval_default_mul_eq {e} {x y} : eval_default e (x * y) = (eval_default e x) * (eval_default e y) :=
+--   by { cases x; cases y; simp [ has_mul.mul, nat_expr.do_mul, nat_expr.eval_default] }
 
 
 -- @[reducible]
 -- def eval : nat_expr -> ℕ 
 --   | (nat_expr.lit n)     := n
---   -- | (nat_expr.var idx)   := match list.nth nat_env idx with | (some (some n)) := n | _ := 0 end
+--   -- | (nat_expr.var idx)   := match List.nth nat_env idx with | (some (some n)) := n | _ := 0 end
 --   | (nat_expr.var idx)   := 0
 --  -- FIXME, maybe use sorry?
 --   | (nat_expr.add e1 e2) := (eval e1) + (eval e2) 
@@ -92,28 +94,28 @@ end nat_expr
 namespace type 
 
 @[reducible]
-def eval (nenv : nat_env) : type -> option type 
+def eval (nenv : nat_env) : type -> Option type 
   | (bv e) := (λn, bv (nat_expr.lit n)) <$> nat_expr.eval nenv e
   | (fn arg res) := fn <$> (eval arg) <*> (eval res)
-  | tp     := return tp
+  | tp     := pure tp
 
 def eval_default (nenv : nat_env) : type -> type 
   | (bv e) := bv (nat_expr.lit (nat_expr.eval_default nenv e))
   | (fn arg res) := fn (eval_default arg) (eval_default res)
   | tp           := tp
 
-def assert_types {m} [monad m] [monad_except string m] 
+def assert_types {m} [Monad m] [MonadExcept String m] 
   (nenv : nat_env) 
-  (t1 t2 : type) : m unit :=
+  (t1 t2 : type) : m Unit :=
   if eval_default nenv t1 = eval_default nenv t2
-  then return () 
-  else throw $ "Type mismatch: " ++ t1.pp ++ " and " ++ t2.pp ++ " in " ++ repr nenv
+  then pure () 
+  else throw $ "Type mismatch: "-- ++ t1.pp ++ " and " ++ t2.pp ++ " in " ++ repr nenv
 
-def assert_bv {m} [monad m] [monad_except string m] (nenv : nat_env) (tp : type) : m ℕ :=
+def assert_bv {m} [Monad m] [MonadExcept String m] (nenv : nat_env) (tp : type) : m ℕ :=
   match tp with
-  | (bv e) := return (nat_expr.eval_default nenv e)
+  | (bv e) := pure (nat_expr.eval_default nenv e)
   | _      := throw "Not a bitvecor"
-  end             
+
 
 end type
 end mc_semantics
@@ -129,21 +131,24 @@ def machine_word := bitvec 64
 
 namespace reg
 
+axiom inject_ax0 : 48 + gpreg_type.width' gpreg_type.reg8h ≤ 64
+axiom inject_ax1 : Π(rtp : gpreg_type), 64 - gpreg_type.width' rtp + gpreg_type.width' rtp ≤ 64
+
 def inject : Π(rtp : gpreg_type), bitvec rtp.width' -> machine_word -> machine_word
   | gpreg_type.reg32 b _   := bitvec.append (bitvec.zero 32) b
-  | gpreg_type.reg8h b old := old.set_bits 48 b (of_as_true trivial)
-  | rtp              b old := old.set_bits (64 - rtp.width') b (begin cases rtp; simp end)
+  | gpreg_type.reg8h b old := old.set_bits 48 b inject_ax0
+  | rtp              b old := old.set_bits (64 - rtp.width') b (inject_ax1 rtp) -- (begin cases rtp; simp end)
 
 def project : Π(rtp : gpreg_type), machine_word -> bitvec rtp.width'
-  | gpreg_type.reg8h b := b.get_bits 48 8 (begin simp [gpreg_type.width'], exact dec_trivial end)
-  | rtp              b := b.get_bits (64 - rtp.width') rtp.width' (begin cases rtp; simp end)
+  | gpreg_type.reg8h b := b.get_bits 48 8 inject_ax0 -- (begin simp [gpreg_type.width'], exact dec_trivial end)
+  | rtp              b := b.get_bits (64 - rtp.width') rtp.width' (inject_ax1 rtp) -- (begin cases rtp; simp end)
 
 end reg
 
 structure machine_state : Type :=
   (mem    : memory)
-  (gpregs : array 16 machine_word)
-  (flags  : array 32 bool)
+  (gpregs : Array machine_word) -- 16
+  (flags  : Array Bool) -- 32
   (ip     : machine_word)
 
 namespace machine_state
@@ -151,43 +156,55 @@ namespace machine_state
 -- Constructs an empty machine state, with 0 where we need a value.
 def empty : machine_state := 
   { mem    := memory.empty
-  , gpregs := mk_array 16 0
-  , flags  := mk_array 32 ff
+  , gpregs := mkArray 16 0
+  , flags  := mkArray 32 false
   , ip     := 0
   }
 
-def get_gpreg  (s : machine_state) (idx : fin 16) : machine_word := array.read s.gpregs idx
+def get_gpreg  (s : machine_state) (idx : Fin 16) : machine_word := 
+  -- FIXME
+  if h : 16 = s.gpregs.size
+  then Array.fget s.gpregs (Eq.recOn h idx) else 0
 
-def update_gpreg (idx : fin 16) (f : machine_word -> machine_word) (s : machine_state) : machine_state :=
-  { s with gpregs := array.write s.gpregs idx (f (get_gpreg s idx)) } 
 
-def get_flag  (s : machine_state) (idx : fin 32) : bool := array.read s.flags idx
 
-def update_flag (idx : fin 32) (f : bool -> bool) (s : machine_state) : machine_state :=
-  { s with flags := array.write s.flags idx (f (get_flag s idx))} 
+def update_gpreg (idx : Fin 16) (f : machine_word -> machine_word) (s : machine_state) : machine_state :=
+  -- FIXME
+  if h : 16 = s.gpregs.size 
+  then { s with gpregs := Array.fset s.gpregs (Eq.recOn h idx) (f (get_gpreg s idx)) }
+  else s 
 
--- def store_bytes (addr : machine_word) (bs : list (bitvec 8)) (s : machine_state) : machine_state := 
+def get_flag  (s : machine_state) (idx : Fin 32) : Bool := 
+  if h : 32 = s.flags.size
+  then Array.fget s.flags (Eq.recOn h idx) else false
+
+def update_flag (idx : Fin 32) (f : Bool -> Bool) (s : machine_state) : machine_state :=
+  if h : 32 = s.flags.size
+  then { s with flags := Array.fset s.flags (Eq.recOn h idx) (f (get_flag s idx)) }
+  else s 
+
+-- def store_bytes (addr : machine_word) (bs : List (bitvec 8)) (s : machine_state) : machine_state := 
 --   { s with mem := s.mem.store_bytes addr bs }
 
--- def read_bytes (s : machine_state) (addr : machine_word) (n : ℕ) : option (list (bitvec 8)) :=
+-- def read_bytes (s : machine_state) (addr : machine_word) (n : ℕ) : Option (List (bitvec 8)) :=
 --   s.mem.read_bytes addr n
 
--- lemma read_bytes_length {s : machine_state} {addr : machine_word} {n : ℕ} {bs : list (bitvec 8)}
+-- lemma read_bytes_length {s : machine_state} {addr : machine_word} {n : ℕ} {bs : List (bitvec 8)}
 --   : read_bytes s addr n = some bs -> bs.length = n := memory.read_bytes_length
 
 def store_word {n : ℕ} (s : machine_state) (addr : machine_word) (b : bitvec (8 * n)) : machine_state := 
   { s with mem := s.mem.store_word addr b }
 
-def read_word (s : machine_state) (addr : machine_word) (n : ℕ) : option (bitvec (8 * n)) :=
+def read_word (s : machine_state) (addr : machine_word) (n : ℕ) : Option (bitvec (8 * n)) :=
   s.mem.read_word addr n
 
-def print_regs (s : machine_state) : string :=
-  let lines := list.zip_with (λn (r : bitvec 64), n ++ ": " ++ r.pp_hex ++ ", ") reg.r64_names s.gpregs.to_list
-  in string.join lines
+def print_regs (s : machine_state) : String :=
+  let lines := List.zipWith (λn (r : bitvec 64), if r = 0 then "" else (n ++ ": " ++ r.pp_hex ++ ", ")) reg.r64_names s.gpregs.toList
+  in String.join lines
 
-def print_set_flags (s : machine_state) : string :=
-  let lines := list.zip_with (λn (r : bool), if r then n else "") reg.flag_names s.flags.to_list
-  in "[" ++ string.intercalate ", " (list.filter (λs, s.length > 0) lines) ++ "]"
+def print_set_flags (s : machine_state) : String :=
+  let lines := List.zipWith (λn (r : Bool), if r then n else "") reg.flag_names s.flags.toList
+  in "[" ++ String.intercalate ", " (List.filter (λs, s.length > 0) lines) ++ "]"
 
 end machine_state
 
@@ -197,31 +214,30 @@ inductive arg_lval
 
 namespace arg_lval
 
-def repr : arg_lval -> string
+def repr : arg_lval -> String
   | (reg r)             := r.repr
-  | (memloc width addr) := has_repr.repr addr ++ "@" ++ has_repr.repr width
+  | (memloc width addr) := HasRepr.repr addr ++ "@" ++ HasRepr.repr width
 
-instance arg_lval_repr : has_repr arg_lval := ⟨repr⟩
+instance arg_lval_repr : HasRepr arg_lval := ⟨repr⟩
 
 end arg_lval
 
 section with_nat_env
 
 -- OS stuff
-parameters (os_state : Type)
+variables (os_state : Type)
 
 structure system_state := 
   (machine_state : machine_state)
   (os_state      : os_state)
 
 @[reducible]
-def system_m := state_t system_state (except string)
-parameter (os_transition : system_m unit)
+def system_m := StateT (system_state os_state) (Except String)
 
-parameter (nenv : nat_env)
+variables (os_transition : system_m os_state Unit) (nenv : nat_env)
 
 @[reducible]
-def eval_nat_expr (e : nat_expr) : nat
+def eval_nat_expr (e : nat_expr) : Nat
   := nat_expr.eval_default nenv e
 
 @[reducible]
@@ -232,18 +248,18 @@ def eval_type : type -> type := type.eval_default nenv
 
 @[reducible]
 def value : type -> Type
-  | (bv e) := bitvec (eval_nat_expr e) -- We use the _normalised_ value here.
-  | bit    := bool
-  | float  := unit -- FIXME
-  | double := unit -- FIXME
-  | x86_80 := unit -- FIXME  
-  | (vec w tp) := array (eval_nat_expr w) (value tp) -- FIXME
+  | (bv e) := bitvec (eval_nat_expr nenv e) -- We use the _normalised_ value here.
+  | bit    := Bool
+  | float  := Unit -- FIXME
+  | double := Unit -- FIXME
+  | x86_80 := Unit -- FIXME  
+  | (vec w tp) := Array /- (eval_nat_expr w) -/ (value tp) -- FIXME
   | (pair tp tp') := value tp × value tp'
   | (fn arg res) := (value arg) -> (value res)
 
 -- namespace value
 
--- def value.repr : Π{tp : type}, value tp -> string
+-- def value.repr : Π{tp : type}, value tp -> String
 --   | (bv e) b                := has_repr.repr b
 --   | (fn _ _ ) _             := "<function>"
 --   | _ _                     := "Unsupported type"
@@ -261,11 +277,11 @@ inductive arg_value
   | natv             : ℕ        -> arg_value 
   -- covers reg, addr, and lhs bindings
   | lval             : arg_lval -> arg_value
-  | rval {tp : type} : value tp -> arg_value
+  | rval {tp : type} : value nenv tp -> arg_value
 
 -- namespace arg_value
 
--- def repr : arg_value -> string 
+-- def repr : arg_value -> String 
 --   | (lval l) := l.repr
 --   | (rval v)  := v.repr
 
@@ -274,36 +290,35 @@ inductive arg_value
 -- end arg_value
 
 @[reducible]
-def environment := list arg_value
+def environment := List (arg_value nenv)
 
 structure evaluator_state : Type :=
-  (system_state : system_state)
-  (environment  : environment) -- read only, but reading can fail
-  (locals       : rbmap ℕ (sigma value))
+  (system_state : system_state os_state)
+  (environment  : environment nenv) -- read only, but reading can fail
+  (locals       : RBMap ℕ (Sigma (value nenv)) (λ(n n' : Nat), decide (n < n')))
 
 -- namespace evaluator_state
 
-def evaluator_state.init (sst : system_state) : evaluator_state := 
+def evaluator_state.init (sst : system_state os_state) : evaluator_state os_state nenv := 
   { system_state  := sst
   , environment   := []
-  , locals        := mk_rbmap ℕ (sigma value)
+  , locals        := {}
   }
 
 -- end evaluator_state
 
 -- Monad for evaluating with failure.  This nesting might be useful to get the ip where things break?
 @[reducible]
-def evaluator := state_t evaluator_state (except string)
+def evaluator := StateT (evaluator_state os_state nenv) (Except String)
 
 -- FIXME: are these an oversight in the stdlib? 
-instance (ε): monad_except ε (except ε) := 
-  { throw := λα e, except.error e, catch := λα m f, match m with | (except.error e) := f e | _ := m end }
+instance (ε): MonadExcept ε (Except ε) := 
+  { throw := λα e, Except.error e, catch := λα m f, match m with | (Except.error e) := f e | _ := m }
 
-instance (ε) (m) [monad_except ε m] : has_orelse m := 
-  { orelse := λα, monad_except.orelse }
+instance (ε) [Inhabited ε] : Alternative (Except ε) := 
+  { failure := λα, Except.error (default ε)
+  , orelse  := λα, MonadExcept.orelse }
 
-instance (ε) [inhabited ε] : alternative (except ε) := 
-  { failure := λα, except.error (default ε)}
 
 -- namespace type
 
@@ -322,27 +337,35 @@ instance (ε) [inhabited ε] : alternative (except ε) :=
 
 -- namespace value
 
-lemma value.type_eval_is_id: Π{tp : type}, value (eval_type tp) = value tp :=
-begin  
-  intros,
-  induction tp,
-  case bv { refl },
-  case fn { simp [value, eval_type, type.eval_default], rw [ tp_ih_arg, tp_ih_res ] },
-  repeat { refl }
-end
+theorem value.type_eval_is_id: Π{tp : type}, value nenv (eval_type nenv tp) = value nenv tp :=
+  I_am_really_sorry _
+-- lemma value.type_eval_is_id: Π{tp : type}, value (eval_type tp) = value tp :=
+-- begin  
+--   intros,
+--   induction tp,
+--   case bv { refl },
+--   case fn { simp [value, eval_type, type.eval_default], rw [ tp_ih_arg, tp_ih_res ] },
+--   repeat { refl }
+-- end
 
-def value.eval_cong {tp tp' : type} (pf : eval_type tp = eval_type tp') (v : value tp) : value tp' :=
-begin
-  rw <- value.type_eval_is_id,
-  rw <- value.type_eval_is_id at v,
-  exact (eq.rec v pf)   
-end
+def value.eval_cong {tp tp' : type} (pf : eval_type nenv tp = eval_type nenv tp') (v : value nenv tp) 
+  : value nenv tp' :=
+  have v' : value nenv (eval_type nenv tp), from Eq.recOn (@value.type_eval_is_id nenv tp).symm v,
+  have v'' : value nenv (eval_type nenv tp'), from Eq.recOn pf v',
+  Eq.recOn (@value.type_eval_is_id nenv tp') v''
+
+
+-- begin
+--   rw <- value.type_eval_is_id,
+--   rw <- value.type_eval_is_id at v,
+--   exact (eq.rec v pf)   
+-- end
 
 -- This allows us to resolve arith in nat_exprs
-def value.type_check {m} [monad m] [monad_except string m] (tp : type) (v : value tp) (tp' : type) 
-  : m (value tp') :=
-  if H : eval_type tp = eval_type tp'
-  then return (value.eval_cong H v)
+def value.type_check {m} [Monad m] [MonadExcept String m] (tp : type) (v : value nenv tp) (tp' : type)
+  : m (value nenv tp') :=
+  if H : eval_type nenv tp = eval_type nenv tp'
+  then pure (value.eval_cong nenv H v)
   else throw "type_check: arg type mismatch"
 
 -- end value
@@ -350,92 +373,93 @@ def value.type_check {m} [monad m] [monad_except string m] (tp : type) (v : valu
 
 -- namespace evaluator
 
-def evaluator.run {a : Type} (m : evaluator a) (s : evaluator_state) : except string (a × evaluator_state) :=
+def evaluator.run {a : Type} (m : evaluator os_state nenv a) (s : evaluator_state os_state nenv) : Except String (a × evaluator_state os_state nenv) :=
   (m.run s)
 
-def evaluator.read_memory_at (addr : machine_word) (n : ℕ) : evaluator (bitvec n) := do
+def evaluator.read_memory_at (addr : machine_word) (n : ℕ) : evaluator os_state nenv (bitvec n) := do
     s <- get, 
     match s.system_state.machine_state.read_word addr (n / 8) with
     | none := throw "read_memory_at: no bytes at addr" 
     | (some w) := 
       if H : 8 * (n / 8) = n
-      then return (bitvec.cong H w)
+      then pure (bitvec.cong H w)
       else throw "evaluator.read_memory_at: width not a multiple of 8"
-    end
+   
 
-def evaluator.map_machine_state (f : machine_state → machine_state) : evaluator unit :=
-  modify (λ(s : evaluator_state), { s with system_state := { s.system_state with machine_state := f s.system_state.machine_state } })
+def evaluator.map_machine_state (f : machine_state → machine_state) : evaluator os_state nenv Unit :=
+  modify (λ(s : evaluator_state os_state nenv), { s with system_state := { s.system_state with machine_state := f s.system_state.machine_state } })
 
-def evaluator.write_memory_at : Π{tp : type} (addr : machine_word) (bytes : value tp), evaluator unit
+def evaluator.write_memory_at : Π{tp : type} (addr : machine_word) (bytes : value nenv tp)
+  , evaluator os_state nenv Unit
   | (bv e) addr bytes :=
-    let width := eval_nat_expr e
+    let width := eval_nat_expr nenv e
     in (if H : width = 8 * (width / 8)
-        then evaluator.map_machine_state (λ(s : machine_state), s.store_word addr (bitvec.cong H bytes))
+        then evaluator.map_machine_state os_state nenv (λ(s : machine_state), s.store_word addr (bitvec.cong H bytes))
         else throw "evaluator.write_memory_at: width not a multiple of 8")
   | _ _ _ := throw "evaluator.write_memory_at not a bv"
 
-def evaluator.arg_at_idx (idx : ℕ) : evaluator arg_value :=
+def evaluator.arg_at_idx (idx : ℕ) : evaluator os_state nenv (arg_value nenv) :=
   do s <- get,
-     match s.environment.nth idx with
-       | (some a) := return a
+     match s.environment.getOpt idx with
+       | (some a) := pure a
        | none     := throw "evaluator.arg_at_idx: no arg at idx"
-     end
 
 -- We should factor out the type check, although it might depend on
 -- the functor (value in this case) if we generalise equality
-def evaluator.local_at_idx (idx : ℕ) (tp : type) : evaluator (value tp) :=
+def evaluator.local_at_idx (idx : ℕ) (tp : type) : evaluator os_state nenv (value nenv tp) :=
   do s <- get,
-     match s.locals.find idx with
-     | (some (sigma.mk tp' v)) := value.type_check _ v tp
-     | none     := throw "local_at_idx: no arg at idx"
-     end
+     (match s.locals.find idx with
+     | (some (Sigma.mk tp' v)) := value.type_check nenv _ v tp
+     | none     := throw "local_at_idx: no arg at idx")
 
-lemma width_width' : Π(rtp : gpreg_type), eval_nat_expr rtp.width = rtp.width' :=
-begin
-  intro, induction rtp; trivial
-end
+theorem width_width' : Π(rtp : gpreg_type), eval_nat_expr nenv rtp.width = rtp.width' :=
+  I_am_really_sorry _
 
-def concrete_reg.set : Π{tp : type}, concrete_reg tp -> value tp -> evaluator unit
+def concrete_reg.set : Π{tp : type}, concrete_reg tp -> value nenv tp -> evaluator os_state nenv Unit
   | ._ (concrete_reg.gpreg idx rtp) b := 
-    let b' : bitvec rtp.width' := eq.rec b (width_width' rtp)
-    in evaluator.map_machine_state (machine_state.update_gpreg idx (reg.inject rtp b'))
+    let b' : bitvec rtp.width' := Eq.rec b (width_width' nenv rtp)
+    in evaluator.map_machine_state os_state nenv (machine_state.update_gpreg idx (reg.inject rtp b'))
   | ._ (concrete_reg.flagreg idx)   b := 
-    evaluator.map_machine_state (machine_state.update_flag idx (λ_, b))
+    evaluator.map_machine_state os_state nenv (machine_state.update_flag idx (λ_, b))
   
-def concrete_reg.from_state : Π{tp : type}, concrete_reg tp -> machine_state -> value tp
+def concrete_reg.from_state : Π{tp : type}, concrete_reg tp -> machine_state 
+  -> value nenv tp
   | _ (concrete_reg.gpreg idx rtp) s := 
-    let v := reg.project rtp (s.get_gpreg idx) 
-    in begin simp [value, width_width' nenv rtp], exact v end
+    let v := reg.project rtp (s.get_gpreg idx) in
+    let v' : bitvec (eval_nat_expr nenv rtp.width) 
+        := Eq.rec v (width_width' nenv rtp).symm
+    in v'
   | _ (concrete_reg.flagreg idx)   s := s.get_flag idx
 
-def concrete_reg.read {tp : type} (r : concrete_reg tp) : evaluator (value tp) := 
+def concrete_reg.read {tp : type} (r : concrete_reg tp) : evaluator os_state nenv (value nenv tp) := 
     do s <- get, 
-       return (concrete_reg.from_state r s.system_state.machine_state)
+       pure (concrete_reg.from_state nenv r s.system_state.machine_state)
 
 -- namespace arg_lval 
 
-def arg_lval.to_value' {m} [monad m] [monad_except string m] 
+def arg_lval.to_value' {m} [Monad m] [MonadExcept String m] 
   (s : machine_state)
-  : arg_lval -> Π(tp : type), m (value tp)
-  | (@arg_lval.reg tp r) tp' := value.type_check tp (concrete_reg.from_state r s) tp'
+  : arg_lval -> Π(tp : type), m (value nenv tp)
+  | (@arg_lval.reg tp r) tp' := 
+    value.type_check nenv tp (concrete_reg.from_state nenv r s) tp'
   | (arg_lval.memloc width addr) tp' :=
     match s.read_word addr (width / 8) with
     | none := throw "arg_lval.to_value': no bytes at addr" 
-    | (some w) := value.type_check (bv (8 * (width / 8))) w tp'
-    end
+    | (some w) := value.type_check nenv (bv (8 * (width / 8))) w tp'
 
-def arg_lval.to_value : arg_lval -> Π(tp : type), evaluator (value tp)
-  | (@arg_lval.reg tp r) tp' := do v <- concrete_reg.read r,
-                                   value.type_check tp v tp'
+def arg_lval.to_value : arg_lval -> Π(tp : type), evaluator os_state nenv (value nenv tp)
+  | (@arg_lval.reg tp r) tp' := do v <- concrete_reg.read os_state nenv r,
+                                   value.type_check nenv tp v tp'
   | (arg_lval.memloc width addr) tp' := do
-    v <- evaluator.read_memory_at addr width,
-    value.type_check (bv width) v tp'
+    v <- evaluator.read_memory_at os_state nenv addr width,
+    value.type_check nenv (bv width) v tp'
 
-def arg_lval.set_value : arg_lval -> Π{tp : type}, value tp -> evaluator unit
-  | (@arg_lval.reg tp r) tp' v := do v' <- value.type_check _ v tp,
-                                     concrete_reg.set r v'
+def arg_lval.set_value : arg_lval -> Π{tp : type}, value nenv tp 
+  -> evaluator os_state nenv  Unit
+  | (@arg_lval.reg tp r) tp' v := do v' <- value.type_check nenv _ v tp,
+                                     concrete_reg.set os_state nenv r v'
   | (arg_lval.memloc _width addr) tp v := do
-    evaluator.write_memory_at addr v
+    evaluator.write_memory_at os_state nenv addr v
 
 -- def read_memory_at (av : arg_value) (n : ℕ) : evaluator (bitvec (8 * n)) :=
 --   match av with 
@@ -444,32 +468,32 @@ def arg_lval.set_value : arg_lval -> Π{tp : type}, value tp -> evaluator unit
 --   end
 
 -- Can fail if types mismatch
-def arg_value.to_value : arg_value -> Π(tp : type), evaluator (value tp)
+def arg_value.to_value : arg_value nenv -> Π(tp : type), evaluator os_state nenv (value nenv tp)
   | (arg_value.natv _ _)  _ := throw "arg_value.to_value: saw a natv"
-  | (arg_value.lval _ l) tp := arg_lval.to_value l tp
-  | (arg_value.rval v) tp := value.type_check _ v tp
+  | (arg_value.lval _ l) tp := arg_lval.to_value os_state nenv l tp
+  | (arg_value.rval v) tp := value.type_check nenv _ v tp
 
-def arg_value.set_value : arg_value -> Π{tp : type}, value tp -> evaluator unit
-  | (arg_value.lval _ l) tp v := arg_lval.set_value l v
+def arg_value.set_value : arg_value nenv -> Π{tp : type}, value nenv tp -> evaluator os_state nenv Unit
+  | (arg_value.lval _ l) tp v := arg_lval.set_value os_state nenv l v
   | _ _ _ := throw "arg_value.set_value: not an lvalue"
 
-def addr.read : Π{tp : type}, addr tp -> evaluator (value tp)
+def addr.read : Π{tp : type}, addr tp -> evaluator os_state nenv (value nenv tp)
   | tp (addr.arg idx) := do 
-      av <- evaluator.arg_at_idx idx,
-      arg_value.to_value av tp -- FIXME: we should really check if this is a memloc first.
+      av <- evaluator.arg_at_idx os_state nenv idx,
+      arg_value.to_value os_state nenv av tp -- FIXME: we should really check if this is a memloc first.
       -- w  <- av.read_memory_at n,
       -- return (value.bv w)
 
-def addr.set : Π{tp : type}, addr tp -> value tp -> evaluator unit
+def addr.set : Π{tp : type}, addr tp -> value nenv tp -> evaluator os_state nenv Unit
   | tp (addr.arg idx) v := do 
-      av <- evaluator.arg_at_idx idx, -- FIXME: we should really check if this is a memloc first.
-      arg_value.set_value av v
+      av <- evaluator.arg_at_idx os_state nenv idx, -- FIXME: we should really check if this is a memloc first.
+      arg_value.set_value os_state nenv av v
 
 -- This is the least-worst option.  The other alternative is to have a
 -- value constructor for functions, which we only need here.
-inductive {u v} hlist {α : Type u} (f : α -> Type v): list α -> Type (max u v)
+inductive {u v} hlist {α : Type u} (f : α -> Type v): List α -> Type (max u v)
   | hnil  : hlist []
-  | hcons {xs : list α} (x : α) : f x -> hlist xs -> hlist (x :: xs)
+  | hcons {xs : List α} (x : α) : f x -> hlist xs -> hlist (x :: xs)
 
 -- namespace nat_expr
 
@@ -496,112 +520,125 @@ inductive {u v} hlist {α : Type u} (f : α -> Type v): list α -> Type (max u v
 -- FIXME: move
 -- Might be easier to define in terms of to_int/from_int etc.
 def bitvec.uext {n} (m : ℕ) (p: n ≤ m) (x:bitvec n) : bitvec m :=
-  bitvec.set_bits 0 0 x (begin simp, exact p end)
+  bitvec.set_bits 0 0 x (I_am_really_sorry _) -- (begin simp, exact p end)
   
 def bitvec.sext {n} (m : ℕ) (p: n ≤ m) (x:bitvec n) : bitvec m :=
-  bitvec.set_bits (if x.msb then (bitvec.zero m).not else 0) 0 x (begin simp, exact p end)
+  bitvec.set_bits (if x.msb then (bitvec.zero m).not else 0) 0 x (I_am_really_sorry _)-- (begin simp, exact p end)
 
 def bitvec.trunc {n} (m : ℕ) (p: m ≤ n) (x:bitvec n) : bitvec m :=
-  bitvec.get_bits x 0 m (begin simp, exact p end)
+  bitvec.get_bits x 0 m (I_am_really_sorry _) --(begin simp, exact p end)
 
-def bit_to_bitvec (n : ℕ) (b : bool) : bitvec n := 
+def bit_to_bitvec (n : ℕ) (b : Bool) : bitvec n := 
   if b then 1 else 0
 
-lemma eval_default_2 {e} : nat_expr.eval_default e 2 = 2 := rfl
+-- lemma eval_default_2 {e} : nat_expr.eval_default e 2 = 2 := rfl
 
-lemma nat_expr_eval_2 : eval_nat_expr 2 = 2 := rfl
+-- lemma nat_expr_eval_2 : eval_nat_expr 2 = 2 := rfl
 
 def type.has_eq : type -> Prop
-  | (bv _)     := true
-  | bit        := true
-  | float      := true 
-  | double     := true 
-  | x86_80     := true
+  | (bv _)     := True
+  | bit        := True
+  | float      := True 
+  | double     := True 
+  | x86_80     := True
   | (vec _ tp) := type.has_eq tp 
   | (pair tp tp') := type.has_eq tp ∧ type.has_eq tp'
-  | (fn _ _)   := false -- could probably come up with something, but nothing efficient
+  | (fn _ _)   := False -- could probably come up with something, but nothing efficient
 
 @[reducible]
-def type.has_eq_dec : Π(tp : type), decidable (type.has_eq tp) 
-  | (bv _)     := is_true true.intro  
-  | bit        := is_true true.intro  
-  | float      := is_true true.intro  
-  | double     := is_true true.intro  
-  | x86_80     := is_true true.intro  
+def type.has_eq_dec : Π(tp : type), Decidable (type.has_eq tp) 
+  | (bv _)     := isTrue True.intro
+  | bit        := isTrue True.intro  
+  | float      := isTrue True.intro  
+  | double     := isTrue True.intro  
+  | x86_80     := isTrue True.intro  
   | (vec _ tp) := type.has_eq_dec tp
-  | (pair tp tp') := @and.decidable _ _ (type.has_eq_dec tp) (type.has_eq_dec tp')
-  | (fn _ _)   := is_false not_false
+  | (pair tp tp') := @And.Decidable _ _ (type.has_eq_dec tp) (type.has_eq_dec tp')
+  | (fn _ _)   := isFalse notFalse
 
-instance decidable_pred_type_has_eq: decidable_pred type.has_eq := type.has_eq_dec
+instance decidable_pred_type_has_eq: DecidablePred type.has_eq := type.has_eq_dec
 
-def value.partial_eq : Π{tp : type}, type.has_eq tp -> value tp -> value tp -> bool
-  | (bv _) _ v1 v2      := (v1 = v2)
+-- set_option trace.eqn_compiler true
+-- set_option trace.debug.eqn_compiler true
+
+-- def tester1 : Π{tp : type}, value nenv tp -> value nenv tp -> Bool
+--   | (bv _)     := λv1 v2, v1 = v2
+--   | _ := λ_ _, true
+
+-- def tester2 : Π{tp : type}, value nenv tp -> value nenv tp -> Bool
+--   | (bv _)     := λv1 v2, v1 - v2 = 0
+--   | _ := λ_ _, true
+
+-- #print tester2._main
+
+def value.partial_eq : Π{tp : type}, type.has_eq tp -> value nenv tp -> value nenv tp -> Bool
+  | (bv _) _ v1 v2      := (v1 - v2 = 0) -- FIXME: bug in the eqn compiler?
   | bit    _ v1 v2      := (v1 = v2)
   | float  _ v1 v2      := (v1 = v2)
   | double  _ v1 v2     := (v1 = v2)
   | x86_80  _ v1 v2     := (v1 = v2)
   | (vec _ tp) pf v1 v2 := 
-    let pf' : type.has_eq tp := pf
-    in (list.zip (array.to_list v1) (array.to_list v2)).all (λ(v : (value tp × value tp)), value.partial_eq pf' v.fst v.snd)
-  | (pair tp tp') pf v1 v2 := 
-    band (value.partial_eq pf.left v1.fst v2.fst) (value.partial_eq pf.right v1.snd v2.snd)
+     let pf' : type.has_eq tp := pf
+     in (List.zip (Array.toList v1) (Array.toList v2)).all (λ(v : (value nenv tp × value nenv tp)), value.partial_eq pf' v.fst v.snd)
+  | (pair tp tp') pf v1 v2 := false -- FIXME
+    -- and (value.partial_eq pf.left v1.fst v2.fst) (value.partial_eq pf.right v1.snd v2.snd)
 
 -- Returns the number of bits that are tt mod 2
-def bitvec.parity {n : ℕ} (b : bitvec n) : bool :=
-  bitvec.foldl bxor ff b
+def bitvec.parity {n : ℕ} (b : bitvec n) : Bool :=
+  bitvec.foldl xor false b
 
-example : bitvec.parity (3 : bitvec 4) = ff := by refl
-example : bitvec.parity (7 : bitvec 4) = tt := by refl
+-- example : bitvec.parity (3 : bitvec 4) = false := by refl
+-- example : bitvec.parity (7 : bitvec 4) = true := by refl
 
-def prim.eval : Π{tp : type}, prim tp -> evaluator (value tp)
+def prim.eval : Π{tp : type}, prim tp -> evaluator os_state nenv (value nenv tp)
   -- `(eq tp)` returns `true` if two values are equal.
   | ._ (prim.eq tp) := 
     if pf : type.has_eq tp 
-    then return (value.partial_eq pf)
+    then pure (value.partial_eq nenv pf)
     else throw "prim.eval.eq: eq at unsupported type"
   -- `(neq tp)` returns `true` if two values are not equal.
   | ._ (prim.neq tp) := 
     if pf : type.has_eq tp 
-    then return (λv1 v2, bnot (value.partial_eq pf v1 v2))
+    then pure (λv1 v2, not (value.partial_eq nenv pf v1 v2))
     else throw "prim.eval.neq: neq at unsupported type"
   -- `(mux tp) c t f` evaluates to `t` when `c` is true and `f` otherwise.
   -- This only evaluates `t` when `c` is true, and only evaluates `f` when
   -- `c` is false.
-  | ._ (prim.mux tp) := return (λb l r, if b then l else r)
+  | ._ (prim.mux tp) := pure (λb l r, if b then l else r)
 
   -- `zero` is the zero bit
-  | ._ prim.bit_zero := return ff
+  | ._ prim.bit_zero := pure false
   -- `one` is the one bit
-  | ._ prim.bit_one := return tt
+  | ._ prim.bit_one := pure true
 
-  | ._ prim.bit_or  := return bor
-  | ._ prim.bit_and := return band
-  | ._ prim.bit_xor := return bxor
+  | ._ prim.bit_or  := pure or
+  | ._ prim.bit_and := pure and
+  | ._ prim.bit_xor := pure xor
 
   -- `bvnat` constructs a bit vector from a natural number.
-  | ._ (prim.bv_nat w n) := return (bitvec.of_nat (eval_nat_expr w) (eval_nat_expr n))
+  | ._ (prim.bv_nat w n) := pure (bitvec.of_nat (eval_nat_expr nenv w) (eval_nat_expr nenv n))
   -- `(add i)` returns the sum of two i-bit numbers.
-  | ._ (prim.add i)        := return bitvec.add
+  | ._ (prim.add i)        := pure bitvec.add
   -- `(adc i)` returns the sum of two i-bit numbers and a carry bit.
-  | ._ (prim.adc i)         := return (λx y b, bitvec.add x (bitvec.add y (bit_to_bitvec _ b)))
-  | ._ (prim.uadc_overflows i) := return (λx y b, bitvec.ult (x + y + bit_to_bitvec (eval_nat_expr i) b) x)
-  | ._ (prim.sadc_overflows i) := return (λx y b, bitvec.slt (x + y + bit_to_bitvec (eval_nat_expr i) b) x)
+  | ._ (prim.adc i)         := pure (λx y b, bitvec.add x (bitvec.add y (bit_to_bitvec _ b)))
+  | ._ (prim.uadc_overflows i) := pure (λx y b, bitvec.ult (x + y + bit_to_bitvec (eval_nat_expr nenv i) b) x)
+  | ._ (prim.sadc_overflows i) := pure (λx y b, bitvec.slt (x + y + bit_to_bitvec (eval_nat_expr nenv i) b) x)
   -- `(bvsub i)` substracts two i-bit bitvectors.
-  | ._ (prim.sub i) := return bitvec.sub
+  | ._ (prim.sub i) := pure bitvec.sub
   -- `(ssbb_overflows i)` true if signed sub overflows, the bit
   -- is a borrow bit.
   -- FIXME: is this correct?
   | ._ (prim.ssbb_overflows i) := 
-    return (λx y b, bitvec.slt x (x - y - bit_to_bitvec (eval_nat_expr i) b))
+    pure (λx y b, bitvec.slt x (x - y - bit_to_bitvec (eval_nat_expr nenv i) b))
   -- `(usbb_overflows i)` true if unsigned sub overflows,
   -- the bit is a borrow bit.
-  | ._ (prim.usbb_overflows i) := return (λx y b, bitvec.ult x (x - y - bit_to_bitvec (eval_nat_expr i) b))
+  | ._ (prim.usbb_overflows i) := pure (λx y b, bitvec.ult x (x - y - bit_to_bitvec (eval_nat_expr nenv i) b))
 
   -- `(neg tp)` Two's Complement negation.
-  | ._ (prim.neg i) := return bitvec.neg
+  | ._ (prim.neg i) := pure bitvec.neg
 
   -- `(mul i)` returns the product of two i-bit numbers.
-  | ._ (prim.mul i)            := return bitvec.mul
+  | ._ (prim.mul i)            := pure bitvec.mul
 
   -- `(quotRem i) n d` returns a pair `(q,r)` where `q` is a `floor (n/d)`
   -- and `r` is `n - d * floor (n/d)`.
@@ -616,98 +653,104 @@ def prim.eval : Π{tp : type}, prim tp -> evaluator (value tp)
   -- triggers a #DE exception when evaluated.
   | ._ (prim.squotRem i) := throw "prim.eval.squotRem unimplemented"
 
-  | ._ (prim.ule i) := return (λx y, bitvec.ule x y)
-  | ._ (prim.ult i) := return (λx y, bitvec.ult x y)
+  | ._ (prim.ule i) := pure (λx y, bitvec.ule x y)
+  | ._ (prim.ult i) := pure (λx y, bitvec.ult x y)
 
   -- `(slice w u l)` takes bits `u` through `l` out of a `w`-bit number.
   --  prim (bv w .→ bv (u+1-l))
   --  slice {w: ℕ} (u l k:ℕ) (H: w = k + (u + 1 - l)) (x: bitvec w) : bitvec (u + 1 - l)
   | tp (prim.slice w u l) := do
-       let n := eval_nat_expr u + 1 - eval_nat_expr l,
-       H <- annotate' "slice" (assert (eval_nat_expr w = (eval_nat_expr w - n + n))),
-       return (begin
-         have rewr : value nenv (bv (u + 1 - l)) = value nenv (bv (nat_expr.lit n)) :=
-           begin simp [n, value, nat_expr.eval_default_sub_eq
-                      , nat_expr.eval_default_add_eq
-                      , eval_nat_expr, nat_expr.eval_default], rw add_comm, refl end,
-         simp [value], rw rewr,
-         exact (bitvec.slice (eval_nat_expr nenv u) (eval_nat_expr nenv l) (eval_nat_expr nenv w - n) H.default)
-        end)
+       let n := eval_nat_expr nenv u + 1 - eval_nat_expr nenv l,
+       H <- annotate' "slice" (assert (eval_nat_expr nenv w = (eval_nat_expr nenv w - n + n))),
+       let f : bitvec (eval_nat_expr nenv w) → bitvec n :=
+         (bitvec.slice (eval_nat_expr nenv u) (eval_nat_expr nenv l) (eval_nat_expr nenv w - n) H.default)
+       in let rewr : value nenv (bv (u + 1 - l)) = value nenv (bv (nat_expr.lit n)) := I_am_really_sorry _ 
+       in pure (λx, Eq.recOn rewr.symm (f x))
+       -- pure (begin
+       --   have rewr : value nenv (bv (u + 1 - l)) = value nenv (bv (nat_expr.lit n)) :=
+       --     begin simp [n, value, nat_expr.eval_default_sub_eq
+       --                , nat_expr.eval_default_add_eq
+       --                , eval_nat_expr, nat_expr.eval_default], rw add_comm, refl end,
+       --   simp [value], rw rewr,
+       --   exact (bitvec.slice (eval_nat_expr nenv u) (eval_nat_expr nenv l) (eval_nat_expr nenv w - n) H.default)
+       --  end)
   -- `(sext i o)` sign extends an `i`-bit number to a `o`-bit number.
-  | ._ (prim.sext i o) := do H <- annotate' "sext" (assert (eval_nat_expr i ≤ eval_nat_expr o)),
-                             return (bitvec.sext (eval_nat_expr o) H.default)
+  | ._ (prim.sext i o) := do H <- annotate' "sext" (assert (eval_nat_expr nenv i ≤ eval_nat_expr nenv o)),
+                             pure (bitvec.sext (eval_nat_expr nenv o) H.default)
   -- `(uext i o)` unsigned extension of an `i`-bit number to a `o`-bit number.
-  | ._ (prim.uext i o) := do H <- annotate' "uext" (assert (eval_nat_expr i ≤ eval_nat_expr o)),
-                             return (bitvec.uext (eval_nat_expr o) H.default)
+  | ._ (prim.uext i o) := do H <- annotate' "uext" (assert (eval_nat_expr nenv i ≤ eval_nat_expr nenv o)),
+                             pure (bitvec.uext (eval_nat_expr nenv o) H.default)
   -- `(trunc i o)` truncates an `i`-bit number to a `o`-bit number.
-  | ._ (prim.trunc i o) := do H <- annotate' "trunc" (assert (eval_nat_expr o ≤ eval_nat_expr i)),
-                              return (bitvec.trunc (eval_nat_expr o) H.default)
+  | ._ (prim.trunc i o) := do H <- annotate' "trunc" (assert (eval_nat_expr nenv o ≤ eval_nat_expr nenv i)),
+                              pure (bitvec.trunc (eval_nat_expr nenv o) H.default)
 
-  | ._ (prim.cat i) := return (λx y, bitvec.cong
-                                    (begin simp [eval_nat_expr, nat_expr.eval_default_mul_eq, nat_expr.eval, eval_default_2, two_mul], 
-                                     end)
-                                    (bitvec.append x y))
+  | ._ (prim.cat i) := pure (λx y, 
+       let prf : eval_nat_expr nenv i + eval_nat_expr nenv i = eval_nat_expr nenv (2 * i) := I_am_really_sorry _
+       in bitvec.cong prf (bitvec.append x y))
+  --(begin simp [eval_nat_expr, nat_expr.eval_default_mul_eq, nat_expr.eval, eval_default_2, two_mul], 
+  --end)
+
   -- | bv_least_nibble (i:ℕ) : prim (bv i .→ bv 4)
-  | ._ (prim.msb i) := return bitvec.msb
-  | ._ (prim.bv_and i) := return bitvec.and
-  | ._ (prim.bv_or i)  := return bitvec.or
-  | ._ (prim.bv_xor i) := return bitvec.xor
-  | ._ (prim.bv_complement i) := return bitvec.not
-  | ._ (prim.shl i)    := return (λx (y : bitvec 8), bitvec.shl x y.to_nat)
+  | ._ (prim.msb i) := pure bitvec.msb
+  | ._ (prim.bv_and i) := pure bitvec.and
+  | ._ (prim.bv_or i)  := pure bitvec.or
+  | ._ (prim.bv_xor i) := pure bitvec.xor
+  | ._ (prim.bv_complement i) := pure bitvec.not
+  | ._ (prim.shl i)    := pure (λx (y : bitvec 8), bitvec.shl x y.to_nat)
   --- `(shl_carry w) c b i` returns the `i`th bit
   --- in the bitvector [c]++b where `i` is treated as an unsigned
   --- number with `0` as the most-significant bit.
   -- e.g., If `i` is `0`, then this returns `c`.  If `i`
   -- exceeds the number of bits in `[c] ++ b` (i.e., i >= w+1),
   -- the the result is false.
-  | ._ (prim.shl_carry w) := return (λc b (i : bitvec 8), 
+  | ._ (prim.shl_carry w) := pure (λc b (i : bitvec 8), 
        match i.to_nat with
-       | nat.zero        := c
+       | Nat.zero        := c
        -- FIXME: is this the intended behaviour?
-       | (nat.succ n) := if n < eval_nat_expr w
-                         then bitvec.nth b (eval_nat_expr w - n - 1) else ff 
-       end)
+       | (Nat.succ n) := if n < eval_nat_expr nenv w
+                         then bitvec.nth b (eval_nat_expr nenv w - n - 1) else false 
+       )
    --- `(shr i) x y` shifts the bits in `x` to the right by
    --- `y` bits where `y` is treated as an unsigned integer.
    --- The new bits shifted in from the right are all zero.
-   | ._ (prim.shr i) := return (λx (y : bitvec 8), bitvec.ushr x y.to_nat)
+   | ._ (prim.shr i) := pure (λx (y : bitvec 8), bitvec.ushr x y.to_nat)
    --- `(shr_carry w) b c i` returns the `i`th bit
    --- in the bitvector b++[c] where `i` is treated as an unsigned
    --- number with `0` as the least-significant bit.
    -- e.g., If `i` is `0`, then this returns `c`.  If `i`
    -- exceeds the number of bits in `b++[c]` (i.e., i >= w+1),
    -- the the result is false.
-  | ._ (prim.shr_carry w) := return (λb c (i : bitvec 8), 
+  | ._ (prim.shr_carry w) := pure (λb c (i : bitvec 8), 
        match i.to_nat with
-       | nat.zero     := c
-       | (nat.succ n) := @ite (n < eval_nat_expr w) (nat.decidable_lt _ _) _ (bitvec.nth b n) ff
--- if n < eval_nat_expr w 
+       | Nat.zero     := c
+       | (Nat.succ n) := @ite (n < eval_nat_expr nenv w) (Nat.decLt _ _) _ (bitvec.nth b n) false
+-- if n < eval_nat_expr nenv w 
 -- then bitvec.nth b n
 -- else ff 
-       end)
+       )
    --- `(sar i) x y` arithmetically shifts the bits in `x` to
    --- the left by `y` bits where `y` is treated as an unsigned integer.
    --- The new bits shifted in all match the most-significant bit in y.
-   | ._ (prim.sar i) := return (λx (y : bitvec 8), bitvec.sshr x y.to_nat)
+   | ._ (prim.sar i) := pure (λx (y : bitvec 8), bitvec.sshr x y.to_nat)
    --- `(sar_carry w) b c i` returns the `i`th bit
    --- in the bitvector b++[c] where `i` is treated as an unsigned
    --- number with `0` as the least-significant bit.
    -- e.g., If `i` is `0`, then this returns `c`.  If `i`
    -- exceeds the number of bits in `b++[c]` (i.e., i >= w+1),
    -- the the result is equal to the most-signfiicant bit.
-   | ._ (prim.sar_carry w) := return (λb c (i : bitvec 8), 
+   | ._ (prim.sar_carry w) := pure (λb c (i : bitvec 8), 
        match i.to_nat with
-       | nat.zero     := c
-       | (nat.succ n) := 
-         @ite (n < eval_nat_expr w) (nat.decidable_lt _ _) _ 
+       | Nat.zero     := c
+       | (Nat.succ n) := 
+         @ite (n < eval_nat_expr nenv w) (Nat.decLt _ _) _ 
               (bitvec.nth b n)
               (bitvec.msb b)
--- (if n < eval_nat_expr w 
+-- (if n < eval_nat_expr nenv w 
 --                           then bitvec.nth b n
 --                           else bitvec.msb b)
-         end)
+         )
    
-  | ._ (prim.even_parity i) := return (λb, bitvec.parity b = ff)
+  | ._ (prim.even_parity i) := pure (λb, bitvec.parity b = false)
   -- `(bsf i)` returns the index of least-significant bit that is 1.
   | ._ (prim.bsf i)         := throw "prim.eval.bsf unimplemented"
   -- `(bsr i)` returns the index of most-significant bit that is 1.
@@ -740,101 +783,100 @@ def prim.eval : Π{tp : type}, prim tp -> evaluator (value tp)
   | ._ prim.x87_fadd           := throw "prim.eval.dx87_fadd unimplemented"
 
   -- Return first element of a pair
-  | ._ (prim.pair_fst x y) := return (λ(v : value x × value y), v.fst)
+  | ._ (prim.pair_fst x y) := pure (λ(v : value nenv x × value nenv y), v.fst)
   -- Return second element of a pair.
-  | ._ (prim.pair_snd x y) := return (λ(v : value x × value y), v.snd)
+  | ._ (prim.pair_snd x y) := pure (λ(v : value nenv x × value nenv y), v.snd)
 
-def value.make_undef : Π(tp : type), value tp 
-  | (bv e) := bitvec.of_nat (eval_nat_expr e) 0
-  | bit    := ff
+def value.make_undef : Π(tp : type), value nenv tp 
+  | (bv e) := bitvec.of_nat (eval_nat_expr nenv e) 0
+  | bit    := false
   | float  := ()
   | double := ()
   | x86_80 := ()
-  | (vec w tp) := mk_array (eval_nat_expr w) (value.make_undef tp)
+  | (vec w tp) := mkArray (eval_nat_expr nenv w) (value.make_undef tp)
   | (pair tp tp') := (value.make_undef tp, value.make_undef tp')
   | (fn arg res) := λ_, value.make_undef res
 
-def expression.eval : Π{tp : type}, expression tp -> evaluator (value tp)
-  | ._ (expression.primitive p) := prim.eval p
+def expression.eval : Π{tp : type}, expression tp -> evaluator os_state nenv (value nenv tp)
+  | ._ (expression.primitive p) := prim.eval os_state nenv p
   | ._ (@expression.bit_test wr wi re idxe) := do
     r   <- expression.eval re,
     idx <- expression.eval idxe,
-    let idx' := idx.to_nat % eval_nat_expr wr 
-    in return (r.nth idx')
+    let idx' := idx.to_nat % eval_nat_expr nenv wr 
+    in pure (r.nth idx')
   | ._ (expression.mulc m xe) := do
     x <- expression.eval xe,
-    return (bitvec.mul (bitvec.of_nat 64 (eval_nat_expr m)) x)
+    pure (bitvec.mul (bitvec.of_nat 64 (eval_nat_expr nenv m)) x)
   | ._ (expression.quotc m xe) := throw "expression.eval.quotc unimplemented"
-  | ._ (expression.undef tp)   := return (value.make_undef tp)
+  | ._ (expression.undef tp)   := pure (value.make_undef nenv tp)
   | ._ (expression.app f a) := (expression.eval f) <*> (expression.eval a)
-  | ._ (expression.get_reg r) := concrete_reg.read r
+  | ._ (expression.get_reg r) := concrete_reg.read os_state nenv r
   | ._ (expression.read tp addre) := do
     addr   <- expression.eval addre,
-    match tp with
-      | (bv we) := evaluator.read_memory_at addr (eval_nat_expr we)
-      | _ := throw "expression.eval.read Trying to store non-bitvector"
-    end
+    (match tp with
+      | (bv we) := evaluator.read_memory_at os_state nenv  addr (eval_nat_expr nenv we)
+      | _ := throw "expression.eval.read Trying to store non-bitvector")
+
   | ._ (expression.streg idx) := throw "expression.eval.streg unimplemented"
-  | ._ (expression.get_local idx tp) := evaluator.local_at_idx idx tp
+  | ._ (expression.get_local idx tp) := evaluator.local_at_idx os_state nenv idx tp
   -- This is overly general, we might not know that av here is an rval
   | ._ (expression.imm_arg idx tp) := do
-    av <- evaluator.arg_at_idx idx,
-    match av with
-    | (arg_value.rval v) := value.type_check _ v tp
-    | _ := throw "expression.eval.imm_arg Not an rval"
-    end
+    av <- evaluator.arg_at_idx os_state nenv idx,
+    (match av with
+    | (arg_value.rval v) := value.type_check nenv _ v tp
+    | _ := throw "expression.eval.imm_arg Not an rval")
+
   | ._ (expression.addr_arg idx) := do
-    av <- evaluator.arg_at_idx idx,
-    match av with
-    | (arg_value.lval _ (arg_lval.memloc _ addr)) := return addr
-    | _ := throw "expression.eval.addr_arg Not an memloc lval"
-    end
+    av <- evaluator.arg_at_idx os_state nenv idx,
+    (match av with
+    | (arg_value.lval _ (arg_lval.memloc _ addr)) := pure addr
+    | _ := throw "expression.eval.addr_arg Not an memloc lval")
   -- FIXME: isn't specific to arg_lval
   | ._ (expression.read_arg idx tp) := do
-    av <- evaluator.arg_at_idx idx,
-    arg_value.to_value av tp
+    av <- evaluator.arg_at_idx os_state nenv idx,
+    arg_value.to_value os_state nenv av tp
 
-def evaluator.set_ip (new_ip : bitvec 64) : evaluator unit :=
-  evaluator.map_machine_state (λ(s : machine_state), { s with ip := new_ip })
+def evaluator.set_ip (new_ip : bitvec 64) : evaluator os_state nenv Unit :=
+  evaluator.map_machine_state os_state nenv (λ(s : machine_state), { s with ip := new_ip })
 
-def lhs.set : Π{tp : type}, lhs tp -> value tp -> evaluator unit
-  | ._ (lhs.set_reg r) v        := concrete_reg.set r v
+def lhs.set : Π{tp : type}, lhs tp -> value nenv tp -> evaluator os_state nenv Unit
+  | ._ (lhs.set_reg r) v        := concrete_reg.set os_state nenv  r v
   | ._ (lhs.write_addr ae tp) v := do
-    a <- expression.eval ae,
-    evaluator.write_memory_at a v
+    a <- expression.eval os_state nenv ae,
+    evaluator.write_memory_at os_state nenv a v
   | ._ (lhs.write_arg idx _tp) v := do
-    av <- evaluator.arg_at_idx idx,
+    av <- evaluator.arg_at_idx os_state nenv idx,
     -- fixme: we ignore tp here?
-    arg_value.set_value av v
+    arg_value.set_value os_state nenv av v
   | ._ (lhs.streg idx) v  := throw "lhs.set: unsupported FP write"
 
-def lhs.read : Π{tp : type}, lhs tp -> evaluator (value tp)
-  | ._ (lhs.set_reg r)        := concrete_reg.read r
+def lhs.read : Π{tp : type}, lhs tp -> evaluator os_state nenv (value nenv tp)
+  | ._ (lhs.set_reg r)        := concrete_reg.read os_state nenv r
   | ._ (lhs.write_addr ae tp) := do
-    addr <- expression.eval ae,
-    match tp with
-      | (bv we) := evaluator.read_memory_at addr (eval_nat_expr we)
-      | _ := throw "lhs.read Trying to store non-bitvector"
-    end
+    addr <- expression.eval os_state nenv ae,
+   (match tp with
+     | (bv we) := evaluator.read_memory_at os_state nenv addr (eval_nat_expr nenv we)
+     | _ := throw "lhs.read Trying to store non-bitvector")
   | ._ (lhs.write_arg idx tp) := do
-    av <- evaluator.arg_at_idx idx,
+    av <- evaluator.arg_at_idx os_state nenv idx,
     -- fixme: we ignore tp here?
-    arg_value.to_value av tp
+    arg_value.to_value os_state nenv av tp
   | ._ (lhs.streg idx) := throw "lhs.set: unsupported FP write"
 
-def evaluator.push64 (v : value (bv 64)) : evaluator unit := do
-  sp <- lhs.read rsp,
+def evaluator.push64 (v : value nenv (bv 64)) : evaluator os_state nenv Unit := do
+  sp <- lhs.read os_state nenv 
+ rsp,
   let sp' := sp - 8 in do
-    lhs.set rsp sp',
-    evaluator.write_memory_at sp' v
+    lhs.set os_state nenv rsp sp',
+    evaluator.write_memory_at os_state nenv sp' v
 
 
 
-def read_cpuid : evaluator unit :=
+def read_cpuid : evaluator os_state nenv Unit :=
   -- Copied from the cpuid results from my macbook
   -- Note: CPUID is allowed to return 0s 
-  let cpuid_values : rbmap ℕ (bitvec 32 × bitvec 32 × bitvec 32 × bitvec 32) :=
-    rbmap.from_list [ (0, (0xd, 0x756e6547, 0x6c65746e, 0x49656e69))
+  let cpuid_values : RBMap ℕ (bitvec 32 × bitvec 32 × bitvec 32 × bitvec 32) (λx y, decide (x < y)) :=
+    RBMap.fromList [ (0, (0xd, 0x756e6547, 0x6c65746e, 0x49656e69))
                     , (1, (0x40661, 0x2100800, 0x7ffafbff, 0xbfebfbff))
                     , (2, (0x76036301, 0xf0b5ff, 0x0, 0xc10000))
                     , (3, (0x0, 0x0, 0x0, 0x0))
@@ -857,46 +899,43 @@ def read_cpuid : evaluator unit :=
                     , (2147483654, (0x0, 0x0, 0x1006040, 0x0))
                     , (2147483655, (0x0, 0x0, 0x0, 0x100))
                     , (2147483656, (0x3027, 0x0, 0x0, 0x0))
-                    ] in -- FIXME: we need to look at rcx sometimes as well
+                    ] (λx y, decide (x < y)) in -- FIXME: we need to look at rcx sometimes as well
     let cpuid_fn (n : ℕ) : (bitvec 32 × bitvec 32 × bitvec 32 × bitvec 32) :=
       match cpuid_values.find n with
       | none     := (0, 0, 0, 0)
       | (some r) := r
-      end
     in do 
-      raxv <- lhs.read rax,
+      raxv <- lhs.read os_state nenv rax,
       match cpuid_fn raxv.to_nat with 
       | (axv, bxv, cxv, dxv) := do 
-        lhs.set eax axv,
-        lhs.set ebx bxv,
-        lhs.set ecx cxv,
-        lhs.set edx dxv
-      end
+        lhs.set os_state nenv eax axv,
+        lhs.set os_state nenv ebx bxv,
+        lhs.set os_state nenv ecx cxv,
+        lhs.set os_state nenv edx dxv
 
-
-def event.eval : event -> evaluator unit
+def event.eval : event -> evaluator os_state nenv Unit
   | event.syscall :=
-    adapt_state (λ(s : evaluator_state), (s.system_state, s))
-                (λs s', { s' with system_state := s })
-                os_transition
+    adaptState (λ(s : evaluator_state os_state nenv), (s.system_state, s))
+               (λs s', { s' with system_state := s })
+               os_transition
   | (event.unsupported msg) := throw ("event.eval: unsupported: " ++ msg)
   | event.pop_x87_register_stack := throw "pop_x87_register_stack"
   | (event.call addr) := do
-    new_ip <- expression.eval addr,
+    new_ip <- expression.eval os_state nenv addr,
     s <- get,
-    evaluator.push64 s.system_state.machine_state.ip,
-    evaluator.set_ip new_ip
+    evaluator.push64 os_state nenv s.system_state.machine_state.ip,
+    evaluator.set_ip  os_state nenv new_ip
 
   | (event.jmp addr) := do
-    new_ip <- expression.eval addr,
-    evaluator.set_ip new_ip
+    new_ip <- expression.eval os_state nenv addr,
+    evaluator.set_ip os_state nenv new_ip
   | (event.branch c addr) := do
-    new_ip <- expression.eval addr,
-    b      <- expression.eval c,
-    when b (evaluator.set_ip new_ip)
+    new_ip <- expression.eval os_state nenv addr,
+    b      <- expression.eval os_state nenv c,
+    when b (evaluator.set_ip os_state nenv new_ip)
   | event.hlt := throw "halt"
   | (event.xchg addr1 addr2) := throw "xchg"
-  | event.cpuid := read_cpuid
+  | event.cpuid := read_cpuid os_state nenv
 
 -- def lhs.read : Π{tp : type}, lhs tp -> evaluator (value tp)
 --   | ._ (lhs.reg r)       := reg.read r
@@ -904,30 +943,31 @@ def event.eval : event -> evaluator unit
 --   | ._ (lhs.arg idx tp)  := do av <- evaluator.arg_at_idx idx, 
 --                                   arg_value.to_value av tp
 --   | ._ (lhs.streg idx)   := throw "lhs.read: unsupported FP read"
-    
-def action.eval : action -> evaluator unit
-  | (action.set l e) := do v <- expression.eval e,
-                           lhs.set l v
+
+def action.eval : action -> evaluator os_state nenv Unit
+  | (action.set l e) := do v <- expression.eval os_state nenv e,
+                           lhs.set os_state nenv l v
   | (action.set_cond l c e) := do
-    b <- expression.eval c,
-    v <- expression.eval e,
-    when b (lhs.set l v)
-  | (@action.set_aligned (bv _) l e align) := do
-    v <- expression.eval e,
-    if v.to_nat % eval_nat_expr align = 0
-    then lhs.set l v
-    else throw "Unaligned set_aligned"
+    b <- expression.eval os_state nenv c,
+    v <- expression.eval os_state nenv e,
+    when b (lhs.set os_state nenv l v)
+  | (@action.set_aligned (bv _) l e align) := throw "set_aligned: buggy case" -- FIXME: compiler bug
+    -- v <- expression.eval os_state nenv e,
+    -- if v.to_nat % eval_nat_expr nenv align = 0
+    -- then lhs.set os_state nenv l v
+    -- else throw "Unaligned set_aligned"
   | (@action.set_aligned _ l e align) := throw "set_aligned: not a bv"
   | (@action.local_def tp idx e) := do 
-    v <- expression.eval e,
-    modify (λs, { s with locals := s.locals.insert idx (sigma.mk tp v)})
-  | (action.event e) := event.eval e
+    v <- expression.eval os_state nenv e,
+    modify (λs, { s with locals := s.locals.insert idx (Sigma.mk tp v)})
+  | (action.event e) := event.eval os_state os_transition nenv e
 
 -- FIXME: check pattern.context |- environment
-def pattern.eval (p : pattern) (e : environment) (s : system_state) : except string system_state :=
+def pattern.eval (p : pattern) (e : environment nenv) (s : system_state os_state) 
+    : Except String (system_state os_state) :=
   -- only machine_state is preserved across instructions
-  let st := { evaluator_state.init s with environment := e }
-  in do (_, s') <- evaluator.run (monad.mapm' action.eval p.actions) st, return s'.system_state
+  let st := { evaluator_state.init os_state nenv s with environment := e }
+  in do (_, s') <- evaluator.run os_state nenv (List.mmap (action.eval os_state os_transition nenv) p.actions >>= λ_, pure ()) st, pure s'.system_state
 
 end with_nat_env
 
