lean/runelf.lean
@@ -1,28 +1,22 @@
 /- This file ties together the evaluator,  elf support, and the decoder -/
 
-import system.io
+-- import system.io
+import galois.init.io
 import x86_semantics.machine_memory
 import .elf
 import .translate
 import decodex86
 
 open x86
-
-def get_filename_arg : io (string × string) := do
-  args ← io.cmdline_args,
-  match args with
-  | [decoder, name ] := do
-      return ( decoder, name )
-  | _ := do
-      io.fail "Usage: CMD decoder elf_file"
-  end
-
--- def evaluate_one (s : machine_state) : (ℕ × sum unknown_byte instruction) -> except string machine_state
+ 
+-- def evaluate_one (s : machine_state) : (ℕ × sum unknown_byte instruction) -> except String machine_state
 --   | (n, sum.inl err)  := throw "Got an unknown byte"
 --   | (n, sum.inr inst) := eval_instruction {s with ip := s.ip + bitvec.of_nat _ n} inst
 
-def get_text_segment (e : elf.ehdr) (phdrs : list (elf.phdr e.elf_class)) : option (elf.phdr e.elf_class) :=
+def get_text_segment (e : elf.ehdr) (phdrs : List (elf.phdr e.elf_class)) : Option (elf.phdr e.elf_class) :=
     phdrs.find (λp, p.flags.has_X)
+
+def throwS { a : Type} (e : String) : IO a := throw (IO.userError e)
 
 namespace sysv_abi
 
@@ -43,12 +37,12 @@ namespace x86_64
 -- For now we just pick a reasonably rsp, initialise s.t. argc == 0
 
 def initialise { ost : Type } (st : system_state ost) : system_state ost :=
-    let rsp_idx := 4 in -- FIXME
+    let rsp_idx : Fin 16 := 4 in -- FIXME
     let stack_top := bitvec.of_nat 64 (2 ^ 47) in
     let words     := [ 0 /- argc -/, 0 /- argv term. -/, 0 /- envp term -/, 0, 0 /- auxv term (2 words) -/ ] in
     let f (acc : (bitvec 64 × machine_state)) (v : ℕ) : bitvec 64 × machine_state :=         
         (acc.fst + bitvec.of_nat _ 8, acc.snd.store_word acc.fst (bitvec.of_nat (8 * 8) v)) in
-    let s'        := list.foldl f (stack_top, st.machine_state) words in
+    let s'        := List.foldl f (stack_top, st.machine_state) words in
     { st with machine_state := machine_state.update_gpreg rsp_idx (λ_, stack_top) s'.snd }
 
 end x86_64
@@ -59,48 +53,47 @@ namespace linux
 namespace x86_64
 open mc_semantics
 
-def rax_idx : fin 16 := 0
+def rax_idx : Fin 16 := 0
 
-def os_state := unit
+def os_state := Unit
 def os_state.empty := ()
 
-def simple_syscall (f : system_state os_state -> machine_word) : system_m os_state unit :=
+def simple_syscall (f : system_state os_state -> machine_word) : system_m os_state Unit :=
   modify (λs, { s with machine_state := s.machine_state.update_gpreg rax_idx (λ_, f s) })
 
-def sys_getuid : system_m os_state unit := 
+def sys_getuid : system_m os_state Unit := 
   let res     := bitvec.of_nat 64 4242
   in simple_syscall (λ_, res)
 
 -- FIXME: maybe use the euid of the current (lean) process?  We could
 -- also forward these to the underlying (Linux) kernel
-def sys_geteuid : system_m os_state unit := 
+def sys_geteuid : system_m os_state Unit := 
   let res     := bitvec.of_nat 64 4242
   in simple_syscall (λ_, res)
 
-def sys_getgid : system_m os_state unit := 
+def sys_getgid : system_m os_state Unit := 
   let res     := bitvec.of_nat 64 4242
   in simple_syscall (λ_, res)
 
 -- FIXME: maybe use the euid of the current (lean) process?  We could
 -- also forward these to the underlying (Linux) kernel
-def sys_getegid : system_m os_state unit := 
+def sys_getegid : system_m os_state Unit := 
   let res     := bitvec.of_nat 64 4242
   in simple_syscall (λ_, res)
 
-def syscalls : rbmap ℕ (system_m os_state unit) := 
-  rbmap.from_list [ (0x66, sys_geteuid)
+def syscalls : RBMap ℕ (system_m os_state Unit) (λx y, decide (x < y)) := 
+  RBMap.fromList [ (0x66, sys_geteuid)
                   , (0x6b, sys_geteuid)
                   , (0x68, sys_getgid)
                   , (0x6c, sys_getegid)
-                  ]
+                  ] (λx y, decide (x < y))
 
-def syscall_handler : system_m os_state unit := do
+def syscall_handler : system_m os_state Unit := do
   s <- get,
   let syscall_no := (s.machine_state.get_gpreg rax_idx).to_nat 
   in match syscalls.find syscall_no with
      | none := throw ("Unknown syscall: " ++ repr syscall_no)
      | (some m) := m
-     end
 
 end x86_64
 end linux
@@ -108,42 +101,47 @@ end linux
 
 -- def lift_eval {α : Type *} |  evaluator α) : io a
 
-def dump_state (s : system_state linux.x86_64.os_state) : io unit := do
+def dump_state (s : system_state linux.x86_64.os_state) : IO Unit := do
   let line := s.machine_state.ip.pp_hex ++ ": " ++ s.machine_state.print_regs ++ " " ++ s.machine_state.print_set_flags
-  in io.put_str_ln line
+  in IO.println line
 
-def decode_loop (d : decodex86.decoder) : ℕ -> system_state linux.x86_64.os_state -> io unit
-  | nat.zero  _     := io.fail "Out of fuel"
-  | (nat.succ n) s  := do
+def decode_loop (d : decodex86.decoder) : ℕ -> system_state linux.x86_64.os_state -> IO Unit
+  | Nat.zero    _   := throw "Out of fuel"
+  | (Nat.succ n) s  := do
   dump_state s,
-  inst <- decodex86.decode d s.machine_state.ip.to_nat,
+  let inst := decodex86.decode d s.machine_state.ip.to_nat in
   match inst with 
-  | (sum.inl err) := io.fail ("Decode error:  " ++ err)
-  | (sum.inr (sum.inl b)) := io.fail ("Unknown byte")
-  | (sum.inr (sum.inr i)) := 
-    match eval_instruction { s with machine_state := { s.machine_state with ip := s.machine_state.ip + bitvec.of_nat _ i.nbytes} } linux.x86_64.syscall_handler i with
-    | (except.error e) := io.fail ("Eval failed: (" ++ repr i ++ ") "  ++ e)
-    | (except.ok s')    := decode_loop n s'
-    end
-  end
+  | (Sum.inl b) := throw ("Unknown byte")
+  | (Sum.inr i) := 
+    (match eval_instruction { s with machine_state := { s.machine_state with ip := s.machine_state.ip + bitvec.of_nat _ i.nbytes} } linux.x86_64.syscall_handler i with
+    | (Except.error e) := throwS ("Eval failed: (" ++ repr i ++ ") "  ++ e)
+    | (Except.ok s')    := decode_loop n s')
 
-def doit : (string × string) -> io unit 
-  | (decoder, elffile) := do
-    ((sigma.mk ehdr phdrs), init_mem) <- elf.read_info_from_file elffile,
-    text_phdr <- match get_text_segment ehdr phdrs with
-                 | none     := io.fail "No executable segment"
-                 | (some p) := return p
-                 end,
-    d <- decodex86.mk_decoder decoder elffile text_phdr.vaddr.val text_phdr.offset.val text_phdr.filesz.val,
-    let init_state := 
-        system_state.mk { machine_state.empty with ip := bitvec.of_nat _ ehdr.entry.val, mem := memory.from_init init_mem } 
-                        linux.x86_64.os_state.empty
-    in
+def doit (elffile : String) : IO Unit := do
+  ((Sigma.mk ehdr phdrs), init_mem) <- elf.read_info_from_file elffile,
+  text_phdr <- (match get_text_segment ehdr phdrs with
+                | none     := throw "No executable segment"
+                | (some p) := pure p),
+  text_bytes <- (match init_mem.lookup_buffer (bitvec.of_nat 64 text_phdr.vaddr.toNat) with
+                | none     := throw "No text region"
+                | some (_, b) := pure b),
+  let entry := ehdr.entry.toNat in do
+  IO.println ("Entry is " ++ repr entry ++ " imm:" ++ repr (18446744073709551616 : Nat) 
+                          ++ " exp:"    ++ repr (2 ^ 64)
+                          ++ " mul:"  ++ repr (9223372036854775808 * 2) ),
+  let d := decodex86.mk_decoder text_bytes text_phdr.vaddr.toNat in
+  let init_state := 
+      system_state.mk { machine_state.empty with 
+                      ip := bitvec.of_nat _ ehdr.entry.toNat
+                      , mem := memory.from_init init_mem } 
+                      linux.x86_64.os_state.empty in
     let init_state_abi := sysv_abi.x86_64.initialise init_state in
     let fuel : ℕ := 100000 in decode_loop d fuel init_state_abi
   
-def main : io unit := 
-  get_filename_arg >>= doit
+def main (xs : List String) : IO UInt32 :=
+  match xs with 
+  | [f] := do doit f, pure 0
+  | _   := throw "Expected a file"
 
 -- set_option profiler true
 -- #eval doit ("../testfiles/two", "../llvm-tablegen-support/llvm-tablegen-support", 1530, 1544)
