lean/translate.lean
@@ -3,41 +3,54 @@
 import x86_semantics.instructions
 import x86_semantics.evaluator
 import decodex86
-import tactic.find
 
 open mc_semantics
 open mc_semantics.type
 
-lemma {u} find_index_lt {α : Type u} (p : α -> Prop) [decidable_pred p] : Π(ls : list α), list.find_index p ls ≤ ls.length := 
-  begin
-    intros,
-    induction ls,
-    { simp [list.find_index] },
-    { simp [list.find_index],
-      by_cases (p ls_hd), 
-        { simp [h] },
-        { simp [h, nat.one_add], apply nat.succ_le_succ, exact ls_ih }
-    }
-  end
+-- lemma {u} find_index_lt {α : Type u} (p : α -> Prop) [decidable_pred p] : Π(ls : list α), list.find_index p ls ≤ ls.length := 
+--   begin
+--     intros,
+--     induction ls,
+--     { simp [list.find_index] },
+--     { simp [list.find_index],
+--       by_cases (p ls_hd), 
+--         { simp [h] },
+--         { simp [h, nat.one_add], apply nat.succ_le_succ, exact ls_ih }
+--     }
+--   end
 
-lemma {u} index_of_lt {α : Type u} [decidable_eq α] (ls : list α) (x : α) 
-  : list.index_of x ls ≤ ls.length := by apply find_index_lt
+-- lemma {u} index_of_lt {α : Type u} [decidable_eq α] (ls : list α) (x : α) 
+--   : list.index_of x ls ≤ ls.length := by apply find_index_lt
+
+namespace List
+
+universe u
+
+protected
+def indexOfAux {α : Type u} [DecidableEq α] (v : α) : Nat -> List α -> Nat
+  | n [] := n
+  | n (x :: xs) := if x = v then n else indexOfAux (n + 1) xs
+
+def indexOf {α : Type u} [DecidableEq α] (xs : List α) (v : α) : Nat := List.indexOfAux v 0 xs
+
+end List
 
 namespace x86
 
 @[reducible]
-def some_gpr := sigma (λ(tp : gpreg_type), concrete_reg (bv tp.width))
+def some_gpr := Sigma (λ(tp : gpreg_type), concrete_reg (bv tp.width))
 
-def register_to_reg (r : decodex86.register) : option some_gpr :=
-  let idx := reg.r64_names.index_of r.top in
+def register_to_reg (r : decodex86.register) : Option some_gpr :=
+  let idx := reg.r64_names.indexOf r.top in
   if H : idx = reg.r64_names.length 
   then none
-  else let idx' := @fin.mk 16 idx (begin
-           destruct (lt_or_eq_of_le (index_of_lt reg.r64_names r.top)); intros Hle,
-           exact Hle,
-           contradiction
-           end)
-       in let mk : Π(tp : gpreg_type), option some_gpr
+  else let prf : idx < 16 := I_am_really_sorry _ in
+       let idx' := @Fin.mk 16 idx prf -- (begin
+           -- destruct (lt_or_eq_of_le (index_of_lt reg.r64_names r.top)); intros Hle,
+           -- exact Hle,
+           -- contradiction
+           -- end)
+       in let mk : Π(tp : gpreg_type), Option some_gpr
                  := λ(tp : gpreg_type), some ⟨tp, concrete_reg.gpreg idx' tp⟩
        in
        match (r.width, r.offset) with 
@@ -47,12 +60,11 @@ def register_to_reg (r : decodex86.register) : option some_gpr :=
          | (32, 0) := mk gpreg_type.reg32
          | (0, 0)  := mk gpreg_type.reg64 -- 0 0 means full reg.     
          | _      := none
-       end
 
 open decodex86
 
-def throw_if {m} {ε} [monad m] [monad_except ε m] (P : Prop) [decidable P] (what : ε) : m unit :=
-  if P then throw what else return ()
+def throw_if {m} {ε} [Monad m] [MonadExcept ε m] (P : Prop) [Decidable P] (what : ε) : m Unit :=
+  if P then throw what else pure ()
 
 -- instance {α : Type} : decidable_pred (@option.is_none α) := 
 --   begin
@@ -72,94 +84,93 @@ def throw_if {m} {ε} [monad m] [monad_except ε m] (P : Prop) [decidable P] (wh
 --     { simp [is_some], apply is_true, constructor}
 --   end
 
-def guard_some {m} [monad m] [monad_except string m] {α β : Type} (reason : string) (x : option α) (f : α -> m β) : m β :=
+def guard_some {m} [Monad m] [MonadExcept String m] {α β : Type} (reason : String) (x : Option α) (f : α -> m β) : m β :=
   match x with 
-  | none := throw (string.append "guard_some: none: " reason)
+  | none := throw (String.append "guard_some: none: " reason)
   | (some y) := f y
-  end
   
-def option_register_to_bv64 {m} [monad m] [monad_except string m] 
+def option_register_to_bv64 {m} [Monad m] [MonadExcept String m] 
   (nenv : nat_env) (s : machine_state)
-  (opt_r : option decodex86.register) : m (bitvec 64) := 
+  (opt_r : Option decodex86.register) : m (bitvec 64) := 
   match opt_r with 
-  | none := return (bitvec.of_nat 64 0)
+  | none := pure (bitvec.of_nat 64 0)
   | (some r) := 
-    if r.top = "rip" 
-    then return s.ip
-    else guard_some "option_register_to_bv64" (register_to_reg r)      
-      (λ(r' : some_gpr),
-        match r' with 
-        | (sigma.mk gpreg_type.reg64 rr) := return (concrete_reg.from_state nenv rr s)
-        | _                              := throw "not a 64bit reg"
-        end) 
-  end
+    (match String.decEq r.top "rip" with -- FIXME: compiler bug with ite?
+     | isTrue _ := pure s.ip
+     | isFalse _ := guard_some "option_register_to_bv64" (register_to_reg r)      
+                    (λ(r' : some_gpr),
+                      match r' with 
+                      | (Sigma.mk gpreg_type.reg64 rr) := pure (concrete_reg.from_state nenv rr s)
+                      | _                              := throw "not a 64bit reg"
+      ))
 
-def operand_to_arg_lval {m} [monad m] [monad_except string m] 
+
+def operand_to_arg_lval {m} [Monad m] [MonadExcept String m] 
     (nenv : nat_env) (s : machine_state) 
     (tp : type) (otp : decodex86.operand_type) : decodex86.operand_value -> m arg_lval
   -- FIXME: check width?
-  | (operand_value.register r) := do sgpr <- guard_some "operand_to_arg_lhs register" (register_to_reg r) return,
+  | (operand_value.register r) := do sgpr <- guard_some "operand_to_arg_lhs register" (register_to_reg r) pure,
                                      assert_types nenv (bv sgpr.fst.width) tp,
-                                     return (arg_lval.reg sgpr.snd)
+                                     pure (arg_lval.reg sgpr.snd)
   -- FIXME: check width?
   | (operand_value.segment opt_r r) := do
-    throw_if (option.is_some opt_r) "got a segment reg",
+    throw_if (Option.isSome opt_r) "got a segment reg",
     -- FIXME: clag
-    sgpr <- guard_some "operand_to_arg_value_lhs register" (register_to_reg r) return,
+    sgpr <- guard_some "operand_to_arg_value_lhs register" (register_to_reg r) pure,
     assert_types nenv (bv sgpr.fst.width) tp,
-    return (arg_lval.reg sgpr.snd)
+    pure (arg_lval.reg sgpr.snd)
   | (operand_value.immediate nbytes val) := throw "operand_to_arg_lval: got an immdiate"
   -- FIXME: we use ip out of the state, we could use the value encoded in the decoded instruction 
   | (operand_value.rel_immediate next_addr nbytes val) := throw "operand_to_arg_lval: got an immdeiate"
   -- base + scale * idx + disp
   | (operand_value.memloc opt_seg opt_base scale opt_idx disp) := do
-    n <- match otp with | (operand_type.mem n) := return n | other := throw "memloc not of mem type" end,
+    n <- match otp with | (operand_type.mem n) := pure n | other := throw "memloc not of mem type",
     assert_types nenv (bv n) tp,
-    throw_if (option.is_some opt_seg) "got a segment reg",
+    throw_if (Option.isSome opt_seg) "got a segment reg",
     b_v   <- option_register_to_bv64 nenv s opt_base,
     idx_v <- option_register_to_bv64 nenv s opt_idx,
-    return (arg_lval.memloc n (b_v + scale * idx_v + disp))
+    pure (arg_lval.memloc n (b_v + scale * idx_v + disp))
 
-def operand_to_arg_value_lhs {m} [monad m] [monad_except string m] 
+def operand_to_arg_value_lhs {m} [Monad m] [MonadExcept String m] 
    (nenv : nat_env) (s : machine_state)
    (tp : type) (op : decodex86.operand) : m (arg_value nenv) :=
    arg_value.lval nenv <$> operand_to_arg_lval nenv s tp op.type op.value
 
-def operand_to_value {m} [monad m] [monad_except string m] 
+def operand_to_value {m} [Monad m] [MonadExcept String m] 
    (nenv : nat_env) (s : machine_state)
    (tp : type) (op : decodex86.operand) : m (value nenv tp) :=
    match op.value with 
      | (operand_value.immediate nbytes val) :=
      -- FIXME: rather than failing here, we will sign extend/truncate.  This may be the wrong approach.
      -- We could also extend operand_type
-       match tp with
-       | (bv e) := return (bitvec.of_int (nat_expr.eval_default nenv e) ((bitvec.of_nat (8 * nbytes) val).to_int))
-       | _      := throw "Immediate should be a bv"
-       end
+       (match tp with
+       | (bv e) := pure (bitvec.of_int (nat_expr.eval_default nenv e) ((bitvec.of_nat (8 * nbytes) val).to_int))
+       | _      := throw "Immediate should be a bv")
+
      -- FIXME: we use ip out of the state, we could use the value encoded in the decoded instruction 
      | (operand_value.rel_immediate next_addr nbytes val) := do
        -- checks for width = 64 bit, basically
        @value.type_check nenv m _ _ (bv 64) (s.ip + bitvec.of_nat _ val) tp
      | _ := do lval <- operand_to_arg_lval nenv s tp op.type op.value,
                arg_lval.to_value' nenv s lval tp
-   end
+
    
-def operand_to_arg_value_expr {m} [monad m] [monad_except string m] 
+def operand_to_arg_value_expr {m} [Monad m] [MonadExcept String m] 
    (nenv : nat_env) (s : machine_state)
    (tp : type) (op : decodex86.operand) : m (arg_value nenv) :=
    arg_value.rval <$> operand_to_value nenv s tp op
 
 def {u v w} first_comb {ε : Type u} {m : Type v → Type w}
-  [monad_except ε m] {α : Type v} (e : ε) (f : ε -> ε -> ε) : list (m α) -> m α
+  [MonadExcept ε m] {α : Type v} (e : ε) (f : ε -> ε -> ε) : List (m α) -> m α
   | []        := throw e
   | [x]       := x
   | (x :: xs) := catch x $ λe1, catch (first_comb xs) $ λe2, throw (f e1 e2)
 
--- Inside the list monad here
-def possible_nat_envs : list binding -> list nat_env
+-- Inside the list Monad here
+def possible_nat_envs : List binding -> List nat_env
   | []                        := [[]]
-  | (binding.one_of ns :: xs) := do n <- ns, e <- possible_nat_envs xs, return (some n :: e)
-  | (_ :: xs)                 := do e <- possible_nat_envs xs, return (none :: e)
+  | (binding.one_of ns :: xs) := do n <- ns, e <- possible_nat_envs xs, pure (some n :: e)
+  | (_ :: xs)                 := do e <- possible_nat_envs xs, pure (none :: e)
 
 /-
 def test_pattern := match mov.patterns with | [x] := x | _ := sorry end
@@ -168,44 +179,44 @@ def test_pattern := match mov.patterns with | [x] := x | _ := sorry end
 -/
 
 def make_environment_helper (nenv : nat_env) (s : machine_state) 
-  : list binding -> list decodex86.operand -> nat_env -> except string (environment nenv) 
-  | [] [] _              := return []
+  : List binding -> List decodex86.operand -> nat_env -> Except String (environment nenv) 
+  | [] [] _              := pure []
   | (binding.one_of _ :: rest) ops (some n :: ns) := do e <- make_environment_helper rest ops ns,
-                                                        return (arg_value.natv nenv n :: e)
+                                                        pure (arg_value.natv nenv n :: e)
   | (binding.reg tp   :: rest) (op :: ops) (_ :: ns) :=
     annotate' "reg" $ do
       av  <- operand_to_arg_value_lhs nenv s tp op,
       -- Mainly to check things are of the right form
-      match av with | (arg_value.lval _ (arg_lval.reg r)) := return () | _ := throw "Not a register" end,
+      match av with | (arg_value.lval _ (arg_lval.reg r)) := pure () | _ := throw "Not a register",
       e   <- make_environment_helper rest ops ns,
-      return (av :: e)
+      pure (av :: e)
 
   | (binding.addr tp   :: rest) (op :: ops) (_ :: ns) :=
     annotate' "addr" $ do
       av  <- operand_to_arg_value_lhs nenv s tp op,
       -- Mainly to check things are of the right form
-      match av with | (arg_value.lval _ (arg_lval.memloc _ _)) := return () | _ := throw "Not a memloc" end,
+      match av with | (arg_value.lval _ (arg_lval.memloc _ _)) := pure () | _ := throw "Not a memloc",
       e   <- make_environment_helper rest ops ns,
-      return (av :: e)
+      pure (av :: e)
 
   | (binding.imm tp   :: rest) (op :: ops) (_ :: ns) :=
     annotate' "imm" $ do
       -- FIXME: check that it is, in fact, an immediate
       av  <- operand_to_arg_value_expr nenv s tp op,
       e   <- make_environment_helper rest ops ns,
-      return (av :: e)
+      pure (av :: e)
 
   | (binding.lhs tp   :: rest) (op :: ops) (_ :: ns) :=
     annotate' "lhs" $ do
       av  <- operand_to_arg_value_lhs nenv s tp op,
       e   <- make_environment_helper rest ops ns,
-      return (av :: e)
+      pure (av :: e)
       
   | (binding.expression tp :: rest) (op :: ops) (_ :: ns) := 
     annotate' "expression" $ do 
       av  <- operand_to_arg_value_expr nenv s tp op,
       e   <- make_environment_helper rest ops ns,
-      return (av :: e)
+      pure (av :: e)
   | _ _ _ := throw "binding/operand mismatch"
 
 /-
@@ -218,49 +229,48 @@ inductive binding
 | expression : type → binding
 -/
 
-def make_environment (s : machine_state) (bindings : list binding) (ops : list decodex86.operand) 
-  : except string (sigma environment) :=
+def make_environment (s : machine_state) (bindings : List binding) (ops : List decodex86.operand) 
+  : Except String (Sigma environment) :=
   first_comb "make_environment: no patterns" (λl r, r) -- l ++ ", " ++ r)
-             (list.map (λnenv, do e <- make_environment_helper nenv s bindings ops nenv, return (sigma.mk nenv e)) (possible_nat_envs bindings))
+             (List.map (λnenv, do e <- make_environment_helper nenv s bindings ops nenv, pure (Sigma.mk nenv e)) (possible_nat_envs bindings))
 
 def instantiate_pattern (s : machine_state) (inst : instruction) (i : decodex86.instruction) 
-  : except string ((sigma environment) × x86.pattern) :=
+  : Except String ((Sigma environment) × x86.pattern) :=
   first_comb "instantiate_pattern: no patterns" (λl r, r) -- l ++ ", " ++ r)
-              (list.map (λ(p : x86.pattern), do e <- make_environment s p.context.bindings.reverse i.operands, return (e, p)) inst.patterns)
+              (List.map (λ(p : x86.pattern), do e <- make_environment s p.context.bindings.reverse i.operands, pure (e, p)) inst.patterns)
 
 -- def eval_simple_instruction (s : instruction) (i : decodex86.instruction) : evaluator environment :=
 --   match s.patterns with
 --   | [p] := do match_context p.context.bindings.reverse i.operands,
 --               s <- get,
---               return s.environment
+--               pure s.environment
 --   | _   := throw "not a simple instruction"
 --   end
 
-def instruction_family (inst : decodex86.instruction) : string :=
-  let (pfx, rest) := list.span char.is_upper inst.mnemonic.to_list in
-  (list.map char.to_lower pfx).as_string
+def instruction_family (inst : decodex86.instruction) : String :=
+  let (pfx, rest) := List.span Char.isUpper inst.mnemonic.toList in
+  (List.map Char.toLower pfx).asString
 
-def instruction_map : rbmap string instruction :=
-  rbmap.from_list (list.map (λ(i : instruction), (i.mnemonic, i)) all_instructions)
+def instruction_map : RBMap String instruction (λx y, decide (x < y)) :=
+  RBMap.fromList (List.map (λ(i : instruction), (i.mnemonic, i)) all_instructions) (λx y, decide (x < y))
 
-def eval_instruction { ost : Type } (s : system_state ost) (sys : system_m ost unit) (i : decodex86.instruction) : except string (system_state ost) :=
+def eval_instruction { ost : Type } (s : system_state ost) (sys : system_m ost Unit) (i : decodex86.instruction) : Except String (system_state ost) :=
   match instruction_map.find (instruction_family i) with               
   | none := throw ("Unknown instruction: " ++ i.mnemonic)
-  | (some inst) := do (sigma.mk nenv env, p) <- annotate' "pattern" (instantiate_pattern s.machine_state inst i),
+  | (some inst) := do (Sigma.mk nenv env, p) <- annotate' "pattern" (instantiate_pattern s.machine_state inst i),
                       annotate' "pattern.eval" (pattern.eval ost sys nenv p env s)
-  end
 
 /- testing -/
-def get_sexp : string -> sexp := λst, 
-    match sexp.from_string st with
-      | (sum.inr s) := s
-      | _           := sexp.list []
-    end
+-- def get_sexp : String -> sexp := λst, 
+--     match sexp.from_string st with
+--       | (sum.inr s) := s
+--       | _           := sexp.list []
+--     end
 
-def string_to_instruction (s : string) : option decodex86.instruction :=
-  decodex86.exec_parser decodex86.parser.instructionp (get_sexp s)
+-- def string_to_instruction (s : String) : Option decodex86.instruction :=
+--   decodex86.exec_parser decodex86.parser.instructionp (get_sexp s)
   
--- def go (s : string) : string := 
+-- def go (s : String) : String := 
 --   match string_to_instruction s with 
 --   | none     := "No parse"
 --   | (some i) := repr i.operands
@@ -274,7 +284,7 @@ def string_to_instruction (s : string) : option decodex86.instruction :=
 
 -- end except
 
--- def go2 (s : string) (si : instruction) : string := 
+-- def go2 (s : String) (si : instruction) : String := 
 --   match string_to_instruction s with 
 --   | none     := "No parse"
 --   | (some i) := match ((eval_simple_instruction si i).run evaluator_state.empty) with
@@ -283,7 +293,7 @@ def string_to_instruction (s : string) : option decodex86.instruction :=
 --                 end
 --   end
 
--- def run_get_rax (s : string) : string :=
+-- def run_get_rax (s : String) : String :=
 --   match string_to_instruction s with 
 --   | none     := "No parse"
 --   | (some i) := match (eval_instruction machine_state.empty i) with
